progress on ed25519

code/experimental/ed25519/Hacl.Impl.Ed25519.SwapConditional.fst
@@ -5,179 +5,309 @@ open FStar.HyperStack
 open FStar.Ghost
 open FStar.Buffer
 
-open Hacl.Bignum.Parameters
-open Hacl.Spec.Bignum.Bigint
 open Hacl.UInt64
+open Hacl.Bignum25519
 open Hacl.Impl.Ed25519.ExtPoint
 
 
 module U32 = FStar.UInt32
 
 
-#reset-options "--initial_fuel 0 --max_fuel 0 --z3rlimit 10"
+#reset-options "--max_fuel 0 --z3rlimit 10"
 
-(* val point : Type0 *)
-(* let point = *)
-(*   let _ = () in *)
-(*   b:buffer limb{length b = 10} *)
+let felem = b:buffer Hacl.UInt64.t{length b = 5}
 
 
-(* (\** Coordinate getters *\) *)
-(* (\* unfold inline_for_extraction val getx: point -> Tot felem *\) *)
-(* (\* unfold inline_for_extraction val gety: point -> Tot felem *\) *)
-(* (\* unfold inline_for_extraction val getz: point -> Tot felem *\) *)
-(* (\* unfold inline_for_extraction let getx p = Buffer.sub p 0ul 5ul *\) *)
-(* (\* unfold inline_for_extraction let gety p = Buffer.sub p 0ul 5ul *\) *)
-(* (\* unfold inline_for_extraction let getz p = Buffer.sub p 5ul 5ul *\) *)
+#reset-options "--max_fuel 0 --z3rlimit 10"
 
-unfold val live_coords: mem -> felem -> felem -> felem -> felem -> GTot Type0
-let live_coords h x y z t =
-  let _ = () in
-  live h x /\ live h z /\ live h y /\ live h t
+private
+val lemma_xor: #n:pos -> a:UInt.uint_t n -> b:UInt.uint_t n -> Lemma
+  (UInt.logxor a (UInt.logxor a b) = b /\ UInt.logxor a (UInt.logxor b a) = b
+    /\ UInt.logxor a (UInt.zero n) = a)
+let lemma_xor #n a b =
+  UInt.logxor_associative a a b;
+  UInt.logxor_commutative a b;
+  UInt.logxor_commutative (UInt.zero n) b;
+  UInt.logxor_self a;
+  UInt.logxor_lemma_1 a;
+  UInt.logxor_lemma_1 b
 
-unfold val live: mem -> point -> GTot Type0
-let live h p =
-  let _ = () in
-  live_coords h (getx p) (gety p) (getz p) (gett p)
-
-(* val make_pre: x:felem -> y:felem -> z:felem -> t:felem -> GTot Type0 *)
-(* let make_pre x y z = *)
-(*   let _ = () in *)
-(*   max_length x == max_length z /\ content x == content z /\ idx z = idx x + length x *)
+private
+val lemma_and: #n:pos -> a:UInt.uint_t n -> Lemma (UInt.logand (UInt.ones n) a = a /\ UInt.logand (UInt.zero n) a = UInt.zero n)
+let lemma_and #n a =
+  UInt.logand_lemma_1 #n a;
+  UInt.logand_lemma_2 #n a;
+  UInt.logand_commutative #n a (UInt.zero n); 
+  UInt.logand_commutative #n a (UInt.ones n)
 
 
-(* unfold inline_for_extraction val make: x:felem -> y:felem -> z:felem{make_pre x y z} -> Tot (p:point) *)
-(* unfold inline_for_extraction let make x y z = join x z *)
-
-#reset-options "--initial_fuel 0 --max_fuel 0 --z3rlimit 100"
-
-private inline_for_extraction val swap_conditional_step: a:felem -> b:felem -> swap:limb{v swap = pow2 64 - 1 \/ v swap = 0} -> ctr:U32.t{U32.v ctr <= len /\ U32.v ctr > 0} ->
+private 
+val swap_conditional_step:
+  out_a:felem -> out_b:felem{disjoint out_a out_b} ->
+  a:felem -> b:felem{disjoint a b} ->
+  swap:limb{v swap = pow2 64 - 1 \/ v swap = 0} ->
   Stack unit
-    (requires (fun h -> disjoint a b /\ Buffer.live h a /\ Buffer.live h b
-      (* /\ Hacl.Spec.EC.AddAndDouble.red_513 (as_seq h a) *)
-      (* /\ Hacl.Spec.EC.AddAndDouble.red_513 (as_seq h b) *)
-    ))
-    (ensures (fun h0 _ h1 -> modifies_2 a b h0 h1 /\ Buffer.live h1 a /\ Buffer.live h1 b
-      /\ Buffer.live h0 a /\ Buffer.live h0 b
-      (* /\ Hacl.Spec.EC.AddAndDouble.red_513 (as_seq h0 a) *)
-      (* /\ Hacl.Spec.EC.AddAndDouble.red_513 (as_seq h0 b) *)
-      (* /\ Hacl.Spec.EC.AddAndDouble.red_513 (as_seq h1 a) *)
-      (* /\ Hacl.Spec.EC.AddAndDouble.red_513 (as_seq h1 b) *)
-      (* /\ (as_seq h1 a, as_seq h1 b) == swap_conditional_step_spec (as_seq h0 a) (as_seq h0 b) swap ctr *)
-    ))
-private inline_for_extraction let swap_conditional_step a b swap ctr =
-  let i = U32.(ctr -^ 1ul) in
-  let ai = a.(i) in
-  let bi = b.(i) in
-  let x = swap &^ (ai ^^ bi) in
-  (* lemma_and (v (ai ^^ bi)); *)
-  cut (v x = v (ai ^^ bi) \/ v x = 0);
-  (* lemma_xor (v ai) (v bi); *)
-  (* lemma_xor (v bi) (v ai);   *)
-  let ai = ai ^^ x in
-  let bi = bi ^^ x in
-  a.(i) <- ai;
-  b.(i) <- bi
+    (requires (fun h -> live h a /\ live h b /\ live h out_a /\ live h out_b))
+    (ensures (fun h0 _ h1 -> modifies_2 out_a out_b h0 h1 /\ live h1 out_a /\ live h1 out_b /\
+      live h0 a /\ live h0 b
+      /\ (if v swap = pow2 64 - 1 then (as_seq h1 out_a == as_seq h0 b /\ as_seq h1 out_b == as_seq h0 a)
+         else (as_seq h1 out_a == as_seq h0 a /\ as_seq h1 out_b == as_seq h0 b)) ))
+#reset-options "--max_fuel 0 --z3rlimit 200"
+let swap_conditional_step a' b' a b swap =
+  let a0 = a.(0ul) in
+  let a1 = a.(1ul) in
+  let a2 = a.(2ul) in
+  let a3 = a.(3ul) in
+  let a4 = a.(4ul) in
+  let b0 = b.(0ul) in
+  let b1 = b.(1ul) in
+  let b2 = b.(2ul) in
+  let b3 = b.(3ul) in
+  let b4 = b.(4ul) in
+  let x0 = swap &^ (a0 ^^ b0) in
+  let x1 = swap &^ (a1 ^^ b1) in
+  let x2 = swap &^ (a2 ^^ b2) in
+  let x3 = swap &^ (a3 ^^ b3) in
+  let x4 = swap &^ (a4 ^^ b4) in
+  lemma_and (v (a0 ^^ b0));
+  lemma_and (v (a1 ^^ b1));
+  lemma_and (v (a2 ^^ b2));
+  lemma_and (v (a3 ^^ b3));
+  lemma_and (v (a4 ^^ b4));
+  assert (v x0 = v (a0 ^^ b0) \/ v x0 = 0);
+  assert (v x1 = v (a1 ^^ b1) \/ v x1 = 0);
+  assert (v x2 = v (a2 ^^ b2) \/ v x2 = 0);
+  assert (v x3 = v (a3 ^^ b3) \/ v x3 = 0);
+  assert (v x4 = v (a4 ^^ b4) \/ v x4 = 0);
+  lemma_xor (v a0) (v b0);
+  lemma_xor (v b0) (v a0);
+  lemma_xor (v a1) (v b1);
+  lemma_xor (v b1) (v a1);
+  lemma_xor (v a2) (v b2);
+  lemma_xor (v b2) (v a2);
+  lemma_xor (v a3) (v b3);
+  lemma_xor (v b3) (v a3);
+  lemma_xor (v a4) (v b4);
+  lemma_xor (v b4) (v a4);
+  let a0' = a0 ^^ x0 in
+  let b0' = b0 ^^ x0 in
+  let a1' = a1 ^^ x1 in
+  let b1' = b1 ^^ x1 in
+  let a2' = a2 ^^ x2 in
+  let b2' = b2 ^^ x2 in
+  let a3' = a3 ^^ x3 in
+  let b3' = b3 ^^ x3 in
+  let a4' = a4 ^^ x4 in
+  let b4' = b4 ^^ x4 in
+  let h0 = ST.get() in
+  Hacl.Lib.Create64.make_h64_5 a' a0' a1' a2' a3' a4';
+  let h1 = ST.get() in
+  Hacl.Lib.Create64.make_h64_5 b' b0' b1' b2' b3' b4';
+  let h2 = ST.get() in
+  no_upd_lemma_1 h1 h2 b' a';
+  Seq.lemma_eq_intro (as_seq h2 a') (if v swap = pow2 64 - 1 then as_seq h0 b else as_seq h0 a);
+  Seq.lemma_eq_intro (as_seq h2 b') (if v swap = pow2 64 - 1 then as_seq h0 a else as_seq h0 b)
 
 
-#reset-options "--initial_fuel 1 --max_fuel 1 --z3rlimit 5"
+#reset-options "--max_fuel 0 --z3rlimit 10"
 
-private val swap_conditional_: a:felem -> b:felem -> swap:limb{v swap = pow2 64 - 1 \/ v swap = 0} -> ctr:U32.t{U32.v ctr <= len} ->
-  Stack unit
-    (requires (fun h -> disjoint a b /\ Buffer.live h a /\ Buffer.live h b
-      (* /\ Hacl.Spec.EC.AddAndDouble.red_513 (as_seq h a) *)
-      (* /\ Hacl.Spec.EC.AddAndDouble.red_513 (as_seq h b) *)
-    ))
-    (ensures (fun h0 _ h1 -> modifies_2 a b h0 h1 /\ Buffer.live h1 a /\ Buffer.live h1 b
-      /\ Buffer.live h0 a /\ Buffer.live h0 b
-      (* /\ Hacl.Spec.EC.AddAndDouble.red_513 (as_seq h0 a) *)
-      (* /\ Hacl.Spec.EC.AddAndDouble.red_513 (as_seq h0 b) *)
-      (* /\ Hacl.Spec.EC.AddAndDouble.red_513 (as_seq h1 a) *)
-      (* /\ Hacl.Spec.EC.AddAndDouble.red_513 (as_seq h1 b) *)
-     (* /\ (as_seq h1 a, as_seq h1 b) == swap_conditional_spec_ (as_seq h0 a) (as_seq h0 b) swap ctr *)
-    ))
-#reset-options "--initial_fuel 1 --max_fuel 1 --z3rlimit 50"
-private let rec swap_conditional_ a b swap ctr =
-  if U32.(ctr =^ 0ul) then ()
-  else (
-    cut (U32.v ctr > 0);
-    swap_conditional_step a b swap ctr;
-    let i = U32.(ctr -^ 1ul) in
-    swap_conditional_ a b swap i
-  )
+private
+inline_for_extraction let mk_mask (iswap:Hacl.UInt64.t{v iswap = 0 \/ v iswap = 1}) :
+  Tot (z:Hacl.UInt64.t{if v iswap = 1 then v z = pow2 64 - 1 else v z = 0})
+  = let swap = 0uL -%^ iswap in
+    assert_norm((0 - 1) % pow2 64 = pow2 64 - 1);
+    assert_norm((0 - 0) % pow2 64 = 0);
+    swap
 
-#reset-options "--initial_fuel 0 --max_fuel 0 --z3rlimit 100"
+
+#reset-options "--max_fuel 0 --z3rlimit 10"
+
+private
+val lemma_point_from_coord: h:mem -> p:point{live h p} ->
+  Lemma (let x = as_seq h (getx p) in let y = as_seq h (gety p) in
+         let z = as_seq h (getz p) in let t = as_seq h (gett p) in
+         as_seq h p == FStar.Seq.(x @| y @| z @| t))
+#reset-options "--max_fuel 0 --z3rlimit 100"
+let lemma_point_from_coord h p =
+  let x = as_seq h (getx p) in let y = as_seq h (gety p) in
+  let z = as_seq h (getz p) in let t = as_seq h (gett p) in
+  Seq.lemma_eq_intro (as_seq h p) FStar.Seq.(x @| y @| z @| t)
+
+
+#reset-options "--max_fuel 0 --z3rlimit 100"
+
+private
+val lemma_point_eq:
+  h:mem -> h':mem -> p:point{live h p} -> p':point{live h' p'} ->
+  Lemma (requires (
+    let x = as_seq h (getx p) in let y = as_seq h (gety p) in
+    let z = as_seq h (getz p) in let t = as_seq h (gett p) in
+    let x' = as_seq h' (getx p') in let y' = as_seq h' (gety p') in
+    let z' = as_seq h' (getz p') in let t' = as_seq h' (gett p') in
+    x == x' /\ y == y' /\ z == z' /\ t == t'))
+        (ensures (as_seq h p == as_seq h' p'))
+let lemma_point_eq h h' p p' =
+  lemma_point_from_coord h p;
+  lemma_point_from_coord h' p';
+  Seq.lemma_eq_intro (as_seq h p) (as_seq h' p')
+
 
 val swap_conditional:
-  a:point ->
-  b:point ->
+  out_a:point -> out_b:point{disjoint out_a out_b} ->
+  a:point{disjoint a out_a /\ disjoint a out_b} ->
+  b:point{disjoint b out_b /\ disjoint b out_a /\ disjoint a b} ->
   i:limb{v i = 0 \/ v i = 1} ->
   Stack unit
-    (requires (fun h -> live h a /\ live h b
-      /\ disjoint (getx a) (getx b) /\ disjoint (getx a) (getz b) /\ disjoint (getx a) (getz a)
-      /\ disjoint (getz a) (getx b) /\ disjoint (getz a) (getz b) /\ disjoint (getx b) (getz b)
-      (* /\ Hacl.Spec.EC.AddAndDouble.red_513 (as_seq h (getx a)) *)
-      (* /\ Hacl.Spec.EC.AddAndDouble.red_513 (as_seq h (getx b)) *)
-      (* /\ Hacl.Spec.EC.AddAndDouble.red_513 (as_seq h (getz a)) *)
-      (* /\ Hacl.Spec.EC.AddAndDouble.red_513 (as_seq h (getz b)) *)
+    (requires (fun h -> live h a /\ live h b /\ live h out_a /\ live h out_b))
+    (ensures (fun h0 _ h1 -> live h0 a /\ live h0 b /\ live h1 out_a /\ live h1 out_b /\
+      modifies_2 out_a out_b h0 h1 /\
+      (if v i = 1 then (as_seq h1 out_a == as_seq h0 b /\ as_seq h1 out_b == as_seq h0 a)
+         else (as_seq h1 out_a == as_seq h0 a /\ as_seq h1 out_b == as_seq h0 b))
     ))
-    (ensures (fun h0 _ h1 -> live h0 a /\ live h0 b /\ modifies_2 a b h0 h1
-      (* /\ Hacl.Spec.EC.AddAndDouble.red_513 (as_seq h0 (getx a)) *)
-      (* /\ Hacl.Spec.EC.AddAndDouble.red_513 (as_seq h0 (getx b)) *)
-      (* /\ Hacl.Spec.EC.AddAndDouble.red_513 (as_seq h0 (getz a)) *)
-      (* /\ Hacl.Spec.EC.AddAndDouble.red_513 (as_seq h0 (getz b)) *)
-      /\ live h1 a /\ live h1 b
-      (* /\ Hacl.Spec.EC.AddAndDouble.red_513 (as_seq h1 (getx a)) *)
-      (* /\ Hacl.Spec.EC.AddAndDouble.red_513 (as_seq h1 (getx b)) *)
-      (* /\ Hacl.Spec.EC.AddAndDouble.red_513 (as_seq h1 (getz a)) *)
-      (* /\ Hacl.Spec.EC.AddAndDouble.red_513 (as_seq h1 (getz b)) *)
-      (* /\ (let spointa1 : spoint_513 = (as_seq h1 (getx a), (as_seq h1 (getz a))) in *)
-      (*    let spointb1 : spoint_513 = (as_seq h1 (getx b), (as_seq h1 (getz b))) in *)
-      (*    (spointa1, spointb1) ==  *)
-      (*     swap_conditional_spec (as_seq h0 (getx a), as_seq h0 (getz a)) (as_seq h0 (getx b), as_seq h0 (getz b)) i) *)
-      ))
-let swap_conditional a b iswap =
-  let swap = limb_zero -%^ iswap in
-  assert_norm((0 - 1) % pow2 64 = pow2 64 - 1);
-  assert_norm((0 - 0) % pow2 64 = 0);
-  swap_conditional_ (getx a) (getx b) swap clen;
-  swap_conditional_ (gety a) (gety b) swap clen;
-  swap_conditional_ (getz a) (getz b) swap clen;
-  swap_conditional_ (gett a) (gett b) swap clen
+
+#reset-options "--max_fuel 0 --z3rlimit 500"
+
+let swap_conditional a' b' a b iswap =
+  let swap = mk_mask iswap in
+  assert(disjoint (getx a) (getx b));
+  assert(disjoint (gety a) (gety b));
+  assert(disjoint (getz a) (getz b));
+  assert(disjoint (gett a) (gett b));
+  assert(disjoint (getx a') (getx b'));
+  assert(disjoint (gety a') (gety b'));
+  assert(disjoint (getz a') (getz b'));
+  assert(disjoint (gett a') (gett b'));
+  let h0 = ST.get() in
+  swap_conditional_step (getx a') (getx b') (getx a) (getx b) swap;
+  let h1 = ST.get() in
+  no_upd_lemma_2 h0 h1 (getx a') (getx b') (getx a);
+  no_upd_lemma_2 h0 h1 (getx a') (getx b') (gety a);
+  no_upd_lemma_2 h0 h1 (getx a') (getx b') (getz a);
+  no_upd_lemma_2 h0 h1 (getx a') (getx b') (gett a);
+  no_upd_lemma_2 h0 h1 (getx a') (getx b') (getx b);
+  no_upd_lemma_2 h0 h1 (getx a') (getx b') (gety b);
+  no_upd_lemma_2 h0 h1 (getx a') (getx b') (getz b);
+  no_upd_lemma_2 h0 h1 (getx a') (getx b') (gett b);
+  swap_conditional_step (gety a') (gety b') (gety a) (gety b) swap;
+  let h2 = ST.get() in
+  no_upd_lemma_2 h1 h2 (gety a') (gety b') (getx a');
+  no_upd_lemma_2 h1 h2 (gety a') (gety b') (getx b');
+  no_upd_lemma_2 h1 h2 (gety a') (gety b') (getx a);
+  no_upd_lemma_2 h1 h2 (gety a') (gety b') (gety a);
+  no_upd_lemma_2 h1 h2 (gety a') (gety b') (getz a);
+  no_upd_lemma_2 h1 h2 (gety a') (gety b') (gett a);
+  no_upd_lemma_2 h1 h2 (gety a') (gety b') (getx b);
+  no_upd_lemma_2 h1 h2 (gety a') (gety b') (gety b);
+  no_upd_lemma_2 h1 h2 (gety a') (gety b') (getz b);
+  no_upd_lemma_2 h1 h2 (gety a') (gety b') (gett b);
+  swap_conditional_step (getz a') (getz b') (getz a) (getz b) swap;
+  let h3 = ST.get() in
+  no_upd_lemma_2 h2 h3 (getz a') (getz b') (getx a');
+  no_upd_lemma_2 h2 h3 (getz a') (getz b') (getx b');
+  no_upd_lemma_2 h2 h3 (getz a') (getz b') (gety a');
+  no_upd_lemma_2 h2 h3 (getz a') (getz b') (gety b');
+  no_upd_lemma_2 h2 h3 (getz a') (getz b') (getx a);
+  no_upd_lemma_2 h2 h3 (getz a') (getz b') (gety a);
+  no_upd_lemma_2 h2 h3 (getz a') (getz b') (getz a);
+  no_upd_lemma_2 h2 h3 (getz a') (getz b') (gett a);
+  no_upd_lemma_2 h2 h3 (getz a') (getz b') (getx b);
+  no_upd_lemma_2 h2 h3 (getz a') (getz b') (gety b);
+  no_upd_lemma_2 h2 h3 (getz a') (getz b') (getz b);
+  no_upd_lemma_2 h2 h3 (getz a') (getz b') (gett b);
+  swap_conditional_step (gett a') (gett b') (gett a) (gett b) swap;
+  let h4 = ST.get() in
+  no_upd_lemma_2 h3 h4 (gett a') (gett b') (getx a');
+  no_upd_lemma_2 h3 h4 (gett a') (gett b') (getx b');
+  no_upd_lemma_2 h3 h4 (gett a') (gett b') (gety a');
+  no_upd_lemma_2 h3 h4 (gett a') (gett b') (gety b');
+  no_upd_lemma_2 h3 h4 (gett a') (gett b') (getz a');
+  no_upd_lemma_2 h3 h4 (gett a') (gett b') (getz b');
+  no_upd_lemma_2 h3 h4 (gett a') (gett b') (getx a);
+  no_upd_lemma_2 h3 h4 (gett a') (gett b') (gety a);
+  no_upd_lemma_2 h3 h4 (gett a') (gett b') (getz a);
+  no_upd_lemma_2 h3 h4 (gett a') (gett b') (gett a);
+  no_upd_lemma_2 h3 h4 (gett a') (gett b') (getx b);
+  no_upd_lemma_2 h3 h4 (gett a') (gett b') (gety b);
+  no_upd_lemma_2 h3 h4 (gett a') (gett b') (getz b);
+  no_upd_lemma_2 h3 h4 (gett a') (gett b') (gett b);
+  lemma_point_eq h4 h0 a' (if v iswap = 1 then b else a);
+  lemma_point_eq h4 h0 b' (if v iswap = 1 then a else b);
+  Seq.lemma_eq_intro (as_seq h4 a') (if v iswap = 1 then as_seq h0 b else as_seq h0 a);
+  Seq.lemma_eq_intro (as_seq h4 b') (if v iswap = 1 then as_seq h0 a else as_seq h0 b)
 
 
-#reset-options "--initial_fuel 0 --max_fuel 0 --z3rlimit 30"
+#reset-options "--max_fuel 0 --z3rlimit 100"
 
-inline_for_extraction val copy:
-  output:point ->
-  input:point ->
+val swap_conditional_inplace:
+  a:point -> b:point{disjoint a b} ->
+  i:limb{v i = 0 \/ v i = 1} ->
   Stack unit
-    (requires (fun h -> live h output /\ live h input
-      /\ disjoint (getx output) (getx input) /\ disjoint (getx output) (getz input)
-      /\ disjoint (getz output) (getx input) /\ disjoint (getz output) (getz input)
-      /\ disjoint (getx output) (getz output)
+    (requires (fun h -> live h a /\ live h b))
+    (ensures (fun h0 _ h1 -> live h0 a /\ live h0 b /\ live h1 a /\ live h1 b /\
+      modifies_2 a b h0 h1 /\
+      (if v i = 1 then (as_seq h1 a == as_seq h0 b /\ as_seq h1 b == as_seq h0 a)
+         else (as_seq h1 a == as_seq h0 a /\ as_seq h1 b == as_seq h0 b))
     ))
-    (ensures (fun h0 _ h1 -> live h0 output /\ live h0 input
-      /\ live h1 output /\ live h1 input
-      /\ modifies_1 output h0 h1
-      /\ disjoint (getx output) (getx input) /\ disjoint (getx output) (getz input)
-      /\ disjoint (getz output) (getx input) /\ disjoint (getz output) (getz input)
-      /\ as_seq h1 (getx output) == as_seq h0 (getx input)
-      /\ as_seq h1 (getz output) == as_seq h0 (getz input)
-    ))
-inline_for_extraction let copy output input =
-  let h = ST.get() in
-  blit (getx input) 0ul (getx output) 0ul clen;
-  blit (gety input) 0ul (gety output) 0ul clen;
-  blit (getz input) 0ul (getz output) 0ul clen;
-  blit (gett input) 0ul (gett output) 0ul clen(* ; *)
-  (* let h' = ST.get() in *)
-  (* Hacl.Spec.Bignum.Fmul.lemma_whole_slice (as_seq h' (getx output)); *)
-  (* Hacl.Spec.Bignum.Fmul.lemma_whole_slice (as_seq h' (getz output)); *)
-  (* Hacl.Spec.Bignum.Fmul.lemma_whole_slice (as_seq h (gety input)); *)
-  (* Hacl.Spec.Bignum.Fmul.lemma_whole_slice (as_seq h (gett input)); *)
-  (* Hacl.Spec.Bignum.Fmul.lemma_whole_slice (as_seq h' (getx output)); *)
-  (* Hacl.Spec.Bignum.Fmul.lemma_whole_slice (as_seq h' (getz output)); *)
-  (* Hacl.Spec.Bignum.Fmul.lemma_whole_slice (as_seq h (gety input)); *)
-  (* Hacl.Spec.Bignum.Fmul.lemma_whole_slice (as_seq h (gett input)) *)
-  
+
+#reset-options "--max_fuel 0 --z3rlimit 500"
+
+let swap_conditional_inplace a b iswap =
+  let swap = mk_mask iswap in
+  assert(disjoint (getx a) (getx b));
+  assert(disjoint (gety a) (gety b));
+  assert(disjoint (getz a) (getz b));
+  assert(disjoint (gett a) (gett b));
+  let h0 = ST.get() in
+  swap_conditional_step (getx a) (getx b) (getx a) (getx b) swap;
+  let h1 = ST.get() in
+  no_upd_lemma_2 h0 h1 (getx a) (getx b) (gety a);
+  no_upd_lemma_2 h0 h1 (getx a) (getx b) (getz a);
+  no_upd_lemma_2 h0 h1 (getx a) (getx b) (gett a);
+  no_upd_lemma_2 h0 h1 (getx a) (getx b) (gety b);
+  no_upd_lemma_2 h0 h1 (getx a) (getx b) (getz b);
+  no_upd_lemma_2 h0 h1 (getx a) (getx b) (gett b);
+  swap_conditional_step (gety a) (gety b) (gety a) (gety b) swap;
+  let h2 = ST.get() in
+  no_upd_lemma_2 h1 h2 (gety a) (gety b) (getx a);
+  no_upd_lemma_2 h1 h2 (gety a) (gety b) (getx b);
+  no_upd_lemma_2 h1 h2 (gety a) (gety b) (getz a);
+  no_upd_lemma_2 h1 h2 (gety a) (gety b) (gett a);
+  no_upd_lemma_2 h1 h2 (gety a) (gety b) (getz b);
+  no_upd_lemma_2 h1 h2 (gety a) (gety b) (gett b);
+  swap_conditional_step (getz a) (getz b) (getz a) (getz b) swap;
+  let h3 = ST.get() in
+  no_upd_lemma_2 h2 h3 (getz a) (getz b) (getx a);
+  no_upd_lemma_2 h2 h3 (getz a) (getz b) (getx b);
+  no_upd_lemma_2 h2 h3 (getz a) (getz b) (gety a);
+  no_upd_lemma_2 h2 h3 (getz a) (getz b) (gety b);
+  no_upd_lemma_2 h2 h3 (getz a) (getz b) (gett a);
+  no_upd_lemma_2 h2 h3 (getz a) (getz b) (gett b);
+  swap_conditional_step (gett a) (gett b) (gett a) (gett b) swap;
+  let h4 = ST.get() in
+  no_upd_lemma_2 h3 h4 (gett a) (gett b) (getx a);
+  no_upd_lemma_2 h3 h4 (gett a) (gett b) (getx b);
+  no_upd_lemma_2 h3 h4 (gett a) (gett b) (gety a);
+  no_upd_lemma_2 h3 h4 (gett a) (gett b) (gety b);
+  no_upd_lemma_2 h3 h4 (gett a) (gett b) (getz a);
+  no_upd_lemma_2 h3 h4 (gett a) (gett b) (getz b);
+  lemma_point_eq h4 h0 a (if v iswap = 1 then b else a);
+  lemma_point_eq h4 h0 b (if v iswap = 1 then a else b);
+  Seq.lemma_eq_intro (as_seq h4 a) (if v iswap = 1 then as_seq h0 b else as_seq h0 a);
+  Seq.lemma_eq_intro (as_seq h4 b) (if v iswap = 1 then as_seq h0 a else as_seq h0 b)
+
+
+#reset-options "--max_fuel 0 --z3rlimit 30"
+
+val copy:
+  output:point ->
+  input:point{disjoint input output} ->
+  Stack unit
+    (requires (fun h -> live h output /\ live h input))
+    (ensures (fun h0 _ h1 -> live h0 output /\ live h0 input /\ live h1 output /\ live h1 input
+      /\ modifies_1 output h0 h1 /\ as_seq h1 output == as_seq h0 input))
+let copy output input =
+  let h  = ST.get() in
+  blit input 0ul output 0ul 20ul;
+  let h' = ST.get() in
+  Seq.lemma_eq_intro (as_seq h input) (Seq.slice (as_seq h input) 0 20);
+  Seq.lemma_eq_intro (as_seq h' output) (Seq.slice (as_seq h' output) 0 20)
