code/experimental/ed25519/Hacl.Impl.Ed25519.Ladder.Step.fst
@@ -1,4 +1,4 @@
-module Hacl.Impl.Ed25519.Ladder.SmallLoop
+module Hacl.Impl.Ed25519.Ladder.Step
 
 
 open FStar.Mul
@@ -47,10 +47,6 @@ let ith_bit k i =
   assert(Hacl.UInt8.v z = (Hacl.UInt8.v kq / pow2 (v r)) % 2);
   z
 
-
-let point_inv h (p:point) : GTot Type0 =
-  live h p /\ (let x = getx p in let y = gety p in let z = getz p in let t = gett p in
-  red_513 (as_seq h x) /\ red_513 (as_seq h y) /\ red_513 (as_seq h z) /\ red_513 (as_seq h t))
 
 
 #reset-options "--max_fuel 0 --z3rlimit 100"
@@ -312,35 +308,35 @@ let loop_step_3 b k ctr i =
   swap_cond nq nqpq nq2 nqpq2 bit
 
 
-val loop_step:
-  b:buffer Hacl.UInt64.t{length b = 80} ->
-  k:uint8_p{length k = 32 /\ disjoint k b} ->
-  ctr:UInt32.t{UInt32.v ctr < 256} ->
-  Stack unit
-    (requires (fun h -> live h b /\ live h k /\
-      (let nq = Buffer.sub b 0ul 20ul in
-       let nqpq = Buffer.sub b 20ul 20ul in
-       let nq2 = Buffer.sub b 40ul 20ul in
-       let nqpq2 = Buffer.sub b 60ul 20ul in
-       point_inv h nq /\ point_inv h nqpq)))
-    (ensures (fun h0 _ h1 -> live h0 b /\ live h0 k /\ live h1 b /\ modifies_1 b h0 h1 /\
-      (let nq = Buffer.sub b 0ul 20ul in
-       let nqpq = Buffer.sub b 20ul 20ul in
-       let nq2 = Buffer.sub b 40ul 20ul in
-       let nqpq2 = Buffer.sub b 60ul 20ul in
-       let ctr' = UInt32.v ctr in
-       let x = as_point h0 nq in
-       let xp1 = as_point h0 nqpq in
-       let x' = as_point h1 nq in
-       let xp1' = as_point h1 nqpq in
-       let x'', xp1'' = Spec.Ed25519.(
-         let x, xp1 = if ith_bit (as_seq h0 k) ctr' = 1 then xp1, x else x, xp1 in
-         let xx = point_double x in
-         let xxp1 = point_add x xp1 in
-         if ith_bit (as_seq h0 k) ctr' = 1 then xxp1, xx else xx, xxp1) in
-       point_inv h0 nq /\ point_inv h0 nqpq /\ point_inv h1 nq /\ point_inv h1 nqpq /\
-       (x'', xp1'') == (x', xp1')
-    )))
+(* val loop_step: *)
+(*   b:buffer Hacl.UInt64.t{length b = 80} -> *)
+(*   k:uint8_p{length k = 32 /\ disjoint k b} -> *)
+(*   ctr:UInt32.t{UInt32.v ctr < 256} -> *)
+(*   Stack unit *)
+(*     (requires (fun h -> live h b /\ live h k /\ *)
+(*       (let nq = Buffer.sub b 0ul 20ul in *)
+(*        let nqpq = Buffer.sub b 20ul 20ul in *)
+(*        let nq2 = Buffer.sub b 40ul 20ul in *)
+(*        let nqpq2 = Buffer.sub b 60ul 20ul in *)
+(*        point_inv h nq /\ point_inv h nqpq))) *)
+(*     (ensures (fun h0 _ h1 -> live h0 b /\ live h0 k /\ live h1 b /\ modifies_1 b h0 h1 /\ *)
+(*       (let nq = Buffer.sub b 0ul 20ul in *)
+(*        let nqpq = Buffer.sub b 20ul 20ul in *)
+(*        let nq2 = Buffer.sub b 40ul 20ul in *)
+(*        let nqpq2 = Buffer.sub b 60ul 20ul in *)
+(*        let ctr' = UInt32.v ctr in *)
+(*        let x = as_point h0 nq in *)
+(*        let xp1 = as_point h0 nqpq in *)
+(*        let x' = as_point h1 nq in *)
+(*        let xp1' = as_point h1 nqpq in *)
+(*        let x'', xp1'' = Spec.Ed25519.( *)
+(*          let x, xp1 = if ith_bit (as_seq h0 k) ctr' = 1 then xp1, x else x, xp1 in *)
+(*          let xx = point_double x in *)
+(*          let xxp1 = point_add x xp1 in *)
+(*          if ith_bit (as_seq h0 k) ctr' = 1 then xxp1, xx else xx, xxp1) in *)
+(*        point_inv h0 nq /\ point_inv h0 nqpq /\ point_inv h1 nq /\ point_inv h1 nqpq /\ *)
+(*        (x'', xp1'') == (x', xp1') *)
+(*     ))) *)
 
 #reset-options "--max_fuel 0 --z3rlimit 1000"
 
